grammatik/Grammatik/Zielsatz/Beweis.lean
@@ -64,6 +64,7 @@ import Grammatik.Zielsatz.Ruhe
 import Grammatik.ZielOrtStart
 import Grammatik.ZielOrtInvGrund
 import Grammatik.Fortschritt
+import Grammatik.Zielsatz.Masken
 
 namespace Gabbro.Grammatik.Zielsatz
 
@@ -144,6 +145,7 @@ theorem ziel_aus (P : Programm D) (S : SperrInv D) (Q : AxEns D) (fs : Aufzaehlu
     keinLogikHalt := main.1.1.2.2.1
     keineVerklemmung := fun hWt => keine_verklemmungG hH.1 hSt sp init hLeer ls.1 ls.2 hr hWt
     keinZyklus := kein_warteZyklusG hH.1 hSt sp init hLeer hr
+    keinKernHalt := kernHaltG_gilt P O passes _ M
     fortschritt := fortschrittG_aus hH.1 hSt sp init (startSpur_nodup_leer init hLeer) hr
       main.1.1.2.2.1
       (bereichG_mehrfaden P O passes Q S fs.1 sp init (kVon P fs.1 init) hH.1 hH.2.1 hH.2.2
